core and !

src/tactic/compute_degree.lean
@@ -165,6 +165,25 @@ meta def eval_guessing (n : ℕ) : expr → tactic ℕ
 | `(max %%a %%b) := do ca ← eval_guessing a, cb ← eval_guessing b, return $ max ca cb
 | e := do cond ← succeeds $ eval_expr ℕ e, if cond then eval_expr ℕ e else pure n
 
+/--  `compute_degree_le_core` differs from `compute_degree_le` simply since it takes a `bool`
+input, instead of parsing a `!` token. -/
+meta def compute_degree_le_core (expos : bool) : tactic unit :=
+do t ← target,
+  try $ refine ``(polynomial.degree_le_nat_degree.trans (with_bot.coe_le_coe.mpr _)),
+  `(polynomial.nat_degree %%tl ≤ %%tr) ← target |
+    fail "Goal is not of the form\n`f.nat_degree ≤ d` or `f.degree ≤ d`",
+  exp_deg ← guess_degree tl >>= eval_guessing 0,
+  cond ← succeeds $ eval_expr ℕ tr,
+  deg_bou ← if cond then eval_expr ℕ tr else pure exp_deg,
+  if deg_bou < exp_deg
+  then fail sformat!"the given polynomial has a term of expected degree\nat least '{exp_deg}'"
+  else
+    repeat $ target >>= resolve_sum_step (if expos then tt else ff),
+    gs ← get_goals,
+    os ← gs.mmap infer_type >>= list.mfilter (λ e, succeeds $ unify t e),
+    guard (os.length = 0) <|> fail "Goal did not change",
+    try $ any_goals' norm_assum
+
 end compute_degree
 
 namespace interactive
@@ -181,21 +200,7 @@ Using `compute_degree_le!` also recurses inside powers.
 Use it only if you know how to prove that exponents of terms other than `X ^ ??` are non-zero!
  -/
 meta def compute_degree_le (expos : parse (tk "!" )?) : tactic unit :=
-do t ← target,
-  try $ refine ``(polynomial.degree_le_nat_degree.trans (with_bot.coe_le_coe.mpr _)),
-  `(polynomial.nat_degree %%tl ≤ %%tr) ← target |
-    fail "Goal is not of the form\n`f.nat_degree ≤ d` or `f.degree ≤ d`",
-  exp_deg ← guess_degree tl >>= eval_guessing 0,
-  cond ← succeeds $ eval_expr ℕ tr,
-  deg_bou ← if cond then eval_expr ℕ tr else pure exp_deg,
-  if deg_bou < exp_deg
-  then fail sformat!"the given polynomial has a term of expected degree\nat least '{exp_deg}'"
-  else
-    repeat $ target >>= resolve_sum_step (if expos.is_some then tt else ff),
-    gs ← get_goals,
-    os ← gs.mmap infer_type >>= list.mfilter (λ e, succeeds $ unify t e),
-    guard (os.length = 0) <|> fail "Goal did not change",
-    try $ any_goals' norm_assum
+if expos.is_some then compute_degree_le_core tt else compute_degree_le_core ff
 
 add_tactic_doc
 { name := "compute_degree_le",
